src/reflection/FStar.Reflection.Constants.fst
@@ -109,6 +109,8 @@ let fstar_refl_optionstate      = mk_refl_types_lid_as_term "optionstate"
 let fstar_refl_optionstate_fv   = mk_refl_types_lid_as_fv   "optionstate"
 let fstar_refl_universe         = mk_refl_types_lid_as_term "universe"
 let fstar_refl_universe_fv      = mk_refl_types_lid_as_fv   "universe"
+let fstar_refl_ctx_uvar_and_subst     = mk_refl_types_lid_as_term "ctx_uvar_and_subst"
+let fstar_refl_ctx_uvar_and_subst_fv  = mk_refl_types_lid_as_fv   "ctx_uvar_and_subst"
 
 (* auxiliary types *)
 let fstar_refl_aqualv           = mk_refl_data_lid_as_term "aqualv"
@@ -146,7 +148,7 @@ let fstar_refl_universe_view_fv = mk_refl_data_lid_as_fv   "universe_view"
 
 (* bv_view, this is a record constructor *)
 
-let ref_Mk_namedv =
+let ref_Mk_namedv_view =
     let lid = fstar_refl_data_lid "Mknamedv_view" in
     let attr = Record_ctor (fstar_refl_data_lid "namedv_view", [
                                 Ident.mk_ident ("uniq" , Range.dummyRange);
@@ -159,7 +161,7 @@ let ref_Mk_namedv =
     ; t   = fv_to_tm fv
     }
 
-let ref_Mk_bv =
+let ref_Mk_bv_view =
     let lid = fstar_refl_data_lid "Mkbv_view" in
     let attr = Record_ctor (fstar_refl_data_lid "view", [
                                 Ident.mk_ident ("index" , Range.dummyRange);
